update  NatSorting.v

CoqScripts/NatSorting.v
@@ -1,6 +1,7 @@
 Require Import Lists.List.
 Import ListNotations.
 Require Import Arith.PeanoNat.
+Require Import Arith.Compare_dec.
 
 
 Inductive sorted : list nat -> Prop :=
@@ -43,3 +44,41 @@ Definition SortSpec :=
   { f : list nat -> list nat  (* функцією, що перетворює список на список     *)
     | (forall lst, same lst (f lst)) /\  (* зберігає склад списку             *)
       (forall lst, sorted (f lst)) }.    (* та утворює відсортований список   *)
+
+Fixpoint aux_ins_sort (n : nat) (lst : list nat) : list nat :=
+  match lst with
+  | [] => [n]
+  | m :: lst' => if le_gt_dec n m then n :: m :: lst'
+                 else m :: (aux_ins_sort n lst')
+  end.
+
+Fixpoint ins_sort (lst : list nat) : list nat :=
+  match lst with
+  | [] => []
+  | n :: lst' => aux_ins_sort n (ins_sort lst')
+  end.
+
+Lemma occnum_aux_ins_sort : forall n m lst,
+  occnum n (aux_ins_sort m lst) = occnum n (m :: lst).
+Admitted.
+
+Lemma aux_ins_sort_inv : 
+
+Theorem ins_sort_is_sorted : SortSpec.
+Proof.
+  exists ins_sort.
+  split.
+  - intro. unfold same. intro.
+    induction lst as [| m lst' IHlst'].
+    + reflexivity.
+    + simpl. rewrite occnum_aux_ins_sort.
+      simpl. destruct (Nat.eq_dec n m) as [E | NE].
+      * rewrite IHlst'. reflexivity.
+      * assumption.
+  - intro.
+    destruct lst as [| n lst'].
+    + constructor.
+    + revert n. induction lst' as [| m lst'' IHlst'']; intro.
+      * constructor. 
+      * destruct (le_gt_dec n m) as [Le | Gt].
+        -- simpl.
